\section{}

We write~$\Ccc'$ instead of~$\Dcc$.

We first note that for any two parallel morphisms~$f, g \colon X \to Y$ in~$\Acat$, it holds that~$f = g$ if and only if~$fx = gx$ for every point~$x \inA X$.
Indeed, we may choose~$x = \id_X \colon X \to X$.
That~$\Hl_n(f) = 0$ is hence~$\Hl_n(f) x = 0$ for every~$x \in \Hl_n(\Ccc)$.

We have for every~$n \in \Integer$ the following commutative diagram:
\[
  \begin{tikzcd}[row sep = huge, column sep = 2.7em]
      C_{n+1}
      \arrow{rr}[above]{d_{n+1}}
      \arrow{dd}[left, near start]{f_{n+1}}
      \arrow[two heads]{dr}[below left]{p}
    & {}
    & C_n
      \arrow{rr}[above]{d_n}
      \arrow{dd}[right, near start]{f_n}
    & {}
    & C_{n-1}
      \arrow{dd}[right, near start]{f_{n-1}}
    & {}
    \\
      {}
    & \Bl_n(\Ccc)
      \arrow[hook]{ur}[above left]{i}
    & {}
    & \Zl_n(\Ccc)
      \arrow[hook']{ul}[above right]{j}
      \arrow[hook,from=ll, dashed, crossing over, "\lambda", near start]
    & {}
    & \Hl_n(\Ccc)
      \arrow[two heads,from=ll, dashed, crossing over, "q", near end]
      \arrow[dashed]{dd}[right]{\Hl_n(f)}
    \\
      C'_{n+1}
      \arrow{rr}[above, near start]{d_{n+1}}
      \arrow[two heads]{dr}[below left]{p'}
    & {}
    & C'_n
      \arrow{rr}[above, near end]{d_n}
    & {}
    & C'_{n-1}
    & {}
    \\
      {}
    & \Bl_n(\Ccc')
      \arrow[hook]{ur}[above left]{i'}
      \arrow[hook,dashed]{rr}[above]{\lambda'}
      \arrow[from=uu, dashed, crossing over, "\Bl_n(f)", near start]
    & {}
    & \Zl_n(\Ccc')
      \arrow[hook']{ul}[above right]{j'}
      \arrow[two heads,dashed]{rr}[above]{q'}
      \arrow[from=uu, dashed, crossing over, "\Zl_n(f)", near start]
    & {}
    & \Hl_n(\Ccc')
  \end{tikzcd}
\]
Let~$s = (s_n)_{n \in \Integer}$ be a null homotopy, i.e.\ let~$s_n \colon C_n \to C'_{n+1}$ be morphisms with
\[
  f_n = d_{n+1} s_n + s_{n-1} d_n
\]
for every~$n \in \Integer$.

We now fix~$n \in \Integer$ and consider~$h_n \inA \Hl_n(\Ccc)$.
There exists~$z_n \inA \Zl_n(\Ccc)$ with~$h_n \equiv q z_n$ because~$q$ is an epimorphism.
Let
\begin{align*}
            c_n
  &\defined j z_n
  \inA      C_n \,,
  \\
            z'_n
  &\defined \Zl_n(f) c_n
  \inA      \Zl_n(\Ccc')  \,,
  \\
            c'_n
  &\defined f_n c_n = f_n j_n z_n = j' \Zl_n(f) c_n = j' z'_n
  \inA      C'_n \,.
\end{align*}
We have that
\[
    d_n c_n
  = d_n j z_n
  = 0
\]
because~$d_n j = 0$.
It therefore follows from the relation~$f_n = d_{n+1} s_n + s_{n-1} d_n$ that
\[
    c'_n
  = f_n c_n
  = (d_{n+1} s_n + s_{n-1} d_n) c_n
  = d_{n+1} s_n c_n + s_{n-1} d_n c_n
  = d_{n+1} s_n c_n \,.
\]
For the points
\begin{align*}
  c'_{n+1}  &\defined s_n c_n \inA C'_{n+1} \,, \\
  b'_n      &\defined p' c'_{n+1} \inA \Bl_n(\Ccc')
\end{align*}
we hence have
\[
    c'_n
  = d_{n+1} c'_{n+1}
  = i' p' c'_{n+1}
  = i' b'_n \,.
\]
It holds that
\[
    \lambda' b'_n
  = z'_n
\]
because
\[
    j' \lambda' b'_n
  = i' b'_n
  = c'_n
  = j' z'_n
\]
and~$j'$ is a monomorphism.
We find overall that
\[
    \Hl_n(f) h_n
  = \Hl_n(f) q z_n
  = q' \Zl_n(f) c_n
  = q' c'_n
  = q' \lambda' b'_n
  = 0
\]
because~$q' \lambda' = 0$.
