\section{}





\subsection*{(i) + (ii)}

Recall that we have for all sets~$X$,~$Y$ and~$Z$ the usual adjuction
\[
  \Maps(X \times Y, Z)
  \xlongrightarrow{\sim}
  \Maps(X, \Maps(Y, Z)) \,,
  \quad
          \mu
  \mapsto [y \mapsto \mu(y,-)]
\]
is a bijection.
It follows in particular that for a~{\kvs}~$V$ we get a bijection
\[
          \Maps(A \times V, V)
  \to     \Maps(A, \Maps(V, V)) \,,
  \quad   \mu
  \mapsto [a \mapsto \mu(a,-)]  \,.
\]
It sufficies to show that~$\mu \in \Maps(A \times V, V)$ is an~{\module{$A$}} structure if and only if the corresponding element~$\varphi \in \Maps(A, \Maps(V,V))$ is a homomorphism of~{\kalg} into~$\End_k(V)$.

The map~$\mu \in \Maps(A \times V, V)$ is an~{\module{$A$}} structure if and only if the following axioms are satisfied for all~$a, a_1, a_2 \in A$, all~$\lambda \in k$ and all~$m, m_1, m_2 \in M$:
\begin{enumerate}[label=(MS\arabic*)]
  \item
    \label{dist second}
    $\mu(a,m_1 + m_2) = \mu(a,m_1) + \mu(a,m_2)$,
  \item
    \label{dist first}
    $\mu(a_1 + a_2,m) = \mu(a_1,m) + \mu(a_2,m)$,
  \item
    \label{ass}
    $\mu(a_1, \mu(a_2, m)) = \mu(a_1 a_2, m)$,
  \item
    \label{unital}
    $\mu(1,m) = m$,
  \item
    \label{kass}
    $\mu(\lambda a, m) = \lambda \mu(a,m) = \mu(a,\lambda m)$.
\end{enumerate}
The map~$\varphi$ is a homomorphism of~{\kalg} into~$\End_k(V)$ if and only if the following conditions are satisfied for all~$a, a_1, a_2 \in A$ and all~$\lambda \in k$:
\begin{enumerate}[label=(AH\arabic*)]
  \item
    $\varphi(a) \in \End_k(M)$,
  \item
    $\varphi(a_1 + a_2) = \varphi(a_1) + \varphi(a_2)$,
  \item
    $\varphi(a_1 a_2) = \varphi(a_1) \varphi(a_2)$,
  \item
    $\varphi(\lambda a) = \lambda \varphi(a)$,
  \item
    $\varphi(1) = \id_V$.
\end{enumerate}
Spelling out these conditions in more detail, we see that the following conditions need to be satisfied for all~$a, a_1, a_2 \in A$, all~$\lambda \in k$ and all~$m, m_1, m_2 \in M$
\begin{enumerate}[label=(AH\arabic**)]
  \item
    \label{new dist second}
    $\varphi(a)(m_1 + m_2) = \varphi(a)(m_1) + \varphi(m_2)$,
  \item
    \label{new kass first}
    $\varphi(a)(\lambda m) = \lambda \varphi(a)(m)$,
  \item
    \label{new dist first}
    $\varphi(a_1 + a_2)(m) = \varphi(a_1)(m) + \varphi(a_2)(m)$,
  \item
    \label{new ass}
    $\varphi(a_1 a_2)(m) = \varphi(a_1)(\varphi(a_2)(m))$,
  \item
    \label{new kass second}
    $\varphi(\lambda a)(m) = \lambda \varphi(a)(m)$,
  \item
    \label{new unital}
    $\varphi(1) = \id_V$.
\end{enumerate}
The relation between~$\mu$ and~$\varphi$ is so that~$\mu(a,m) = \varphi(a)(m)$ for all~$a \in A$ and all~$m \in M$.
We therefore find that condition~\ref{dist second} is equivalent to~\ref{new dist second},~\ref{dist first} is equivalent to~\ref{new dist first},~\ref{ass} is equivalent to~\ref{new ass},~\ref{unital} is equivalent to~\ref{new unital}, and~\ref{kass} is equivalent to the combination of~\ref{new kass first} and~\ref{new kass second}.





\addtocounter{subsection}{2}
\subsection{}

Since the map~$f$ is already~{\klin}, we find that
\begin{align*}
      &{} \text{$f$ is a homomorphism of~{\module{$A$}}} \\
  \iff&{} \text{$f(av) = af(v)$ for all~$a \in A$,~$v \in V$} \\
  \iff&{} \text{$f(\varphi(a)) = \psi(a)(f(v)$ for all~$a \in A$,~$v \in V$}  \\
  \iff&{} \text{$f \circ \varphi(a) = \psi(a) \circ f$ for all~$a \in A$} \,.
\end{align*}




