\section{}

Let~$p \colon X \times Y' \to X$ and~$q \colon X \times Y' \to Y'$ be the canonical projections belonging to the biproduct~$X \otimes Y'$
Let~$k \colon X' \to X \times Y'$ be a kernel of the morphism
\[
            d
  \defined  f \circ p - g \circ q
  \colon    X \times Y'
  \to       Y \,.
\]
For~$f' \defined q \circ k$ and~$g' \defined q \circ k$ we then have the following diagram, in which the upper and left triangles commute:
\[
  \begin{tikzcd}
      X'
      \arrow{rr}[above]{g'}
      \arrow{dr}[below left]{k}
      \arrow{dd}[right]{f'}
    & {}
    & X
      \arrow{dd}[right]{f}
    \\
      {}
    & X \times Y'
      \arrow{ur}[below right]{p}
      \arrow{dr}[above right]{d}
      \arrow{dl}[below right]{q}
    & {}
    \\
      Y'
      \arrow{rr}[above]{g}
    & {}
    & Y
  \end{tikzcd}
\]
The outer square also commutes because
\[
    0
  = d \circ k
  = (f \circ p - g \circ c) \circ k
  = f \circ p \circ k - g \circ q \circ k
  = f \circ g' - g \circ f'
\]
and hence~$f \circ g' - g \circ f'$.

If more generally~$Z \in \Ob(\Ccat)$ is an object and~$\alpha \colon Z \to X$ and~$\beta \colon Z \to Y'$ are morphisms, with~$f \circ \alpha = g \circ \beta$ then it holds for the morphism~$(\alpha,\beta) \colon Z \to X \times Y$ that
\begin{align*}
      d \circ (\alpha,\beta)
  &=  (f \circ p - g \circ q) \circ (\alpha,\beta)  \\
  &=  f \circ p \circ (\alpha,\beta) - g \circ q \circ (\alpha,\beta)
   =  f \circ \alpha - g \circ \beta
   =  0 \,.
\end{align*}
Hence~$(\alpha, \beta)$ factors uniquely through the kernel~$k \colon X' \to X \times Y'$ of~$d$, i.e.\ there exists a unique morphism~$\gamma \colon Z \to X'$ with~$k \circ \gamma = (\alpha, \beta)$.
\[
  \begin{tikzcd}[column sep={6em,between origins}]
      Z
      \arrow[bend left]{drrr}[above right]{\alpha}
      \arrow[bend right]{dddr}[below left]{\beta}
      \arrow[dashed]{dr}[below left]{\gamma}
    & {}
    & {}
    & {}
    \\
      {}
    & X'
      \arrow{rr}[above]{g'}
      \arrow{dr}[below left]{k}
      \arrow{dd}[right]{f'}
    & {}
    & X
      \arrow{dd}[right]{f}
    \\
      {}
    & {}
    & X \times Y'
      \arrow[dashed, from=uull, bend left, crossing over, above right, "{(\alpha,\beta)}"]
      \arrow{ur}[below right]{p}
      \arrow{dr}[above right]{d}
      \arrow{dl}[below right]{q}
    & {}
    \\
      {}
    & Y'
      \arrow{rr}[above]{g}
    & {}
    & Y
  \end{tikzcd}
\]
It then holds that
\begin{gather*}
    g' \circ \gamma
  = p \circ k \circ \gamma
  = p \circ (\alpha, \beta)
  = \alpha
\intertext{and}
    f' \circ \gamma
  = q \circ k \circ \gamma
  = q \circ (\alpha, \beta)
  = \beta \,.
\end{gather*}

Suppose on the other hand that~$\gamma' \colon Z \to X'$ is another morphism which makes the diagram
\[
  \begin{tikzcd}
      Z
      \arrow[bend left]{drr}[above right]{\alpha}
      \arrow[bend right]{ddr}[below left]{\beta}
      \arrow{dr}[above right]{\gamma}
    & {}
    & {}
    \\
      {}
    & X'
      \arrow{r}[above]{g'}
      \arrow{d}[right]{f'}
    & X
      \arrow{d}[right]{f}
    \\
      {}
    & Y'
      \arrow{r}[above]{g}
    & Y
  \end{tikzcd}
\]
commute.
Then the composition~$k \circ \gamma'$ satisfies
\begin{gather*}
    p \circ k \circ \gamma'
  = g' \circ \gamma'
  = \alpha
\shortintertext{and}
    q \circ k \circ \gamma'
  = f' \circ \gamma'
  = \beta \,,
\end{gather*}
and is hence given by~$k \circ \gamma' = (\alpha, \beta)$.
It follows that~$\gamma = \gamma'$ by the uniqueness of~$\gamma$.




