\section{}
We abbreviate~$H_n \defined \Hl(V_\bullet)$,~$Z_n \defined \Zl(V_\bullet)$ and~$B_n \defined \Bl(V_\bullet)$ for every~$n \in \Integer$.

We have for every~$n \in \Integer$ that
\[
    \dim H_n
  = \dim Z_n/B_n
  = \dim Z_n - \dim B_n \,,
\]
and also that
\[
    \dim V_n
  = \dim Z_n + \dim B_{n-1} \,.
\]
We hence find that
\begin{align*}
      \sum_n (-1)^n \dim V_n
  &=  \sum_n (-1)^n (\dim Z_n + \dim B_{n-1}) \\
  &=  \sum_n (-1)^n \dim Z_n + \sum_n (-1)^n \dim B_{n-1} \\
  &=  \sum_n (-1)^n \dim Z_n - \sum_n (-1)^n \dim B_n \\
  &=  \sum_n (-1)^n (\dim Z_n - \dim B_n) \\
  &=  \sum_n (-1)^n \dim H_n \,.
\end{align*}




