\section{}

If the functor~$G \colon \Dcat \to \Ccat$ admits a left adjoint functor~$F \colon \Ccat \to \Dcat$  then
\[
        \Ccat(X, G(-))
  \cong \Dcat(F(X), -) \,,
\]
for every~$X \in \Ob(\Ccat)$, which shows that the functor~$\Ccat(X, G(-))$ is represented by the object~$F(X) \in \Ob(\Dcat)$.

Suppose on the other hand that the functor~$\Ccat(X, G(-)) \colon \Dcat \to \Set$ is representable for every object~$X \in \Ob(\Ccat)$.
Let~$\Ecat \subseteq \Fun(\Dcat, \Set)$ be the the essential image of the Yoneda embedding
\[
          E
  \colon  \Dcat
  \to     \Fun(\Dcat, \Set) \,,
\]
i.e.\ the full subcategory of~$\Fun(\Dcat, \Set)$ spanned by all representable functors.
It follows from the Yoneda embedding~$E$ being fully faithful and essentially surjective (onto~$\Ecat$) that there exist a \dash{quasi}{inverse}~$E' \colon \Ecat \to \Dcat$ for~$E$.
Note that both~$E$ and~$E'$ are contravariant.

We can now define a functor
\[
          F'
  \colon  \Ccat
  \to     \Fun(\Dcat, \Set)
\]
which assigns to every objects~$X \in \Ob(\Ccat)$ the functor
\[
            F'(X)
  \defined  \Ccat(X, G(-))
  \colon    \Dcat
  \to       \Set \,,
\]
and assigns to every morphism~$f \colon X \to X'$ in~$\Ccat$ the natural transformation
\[
            F'(f)
  \defined  f^*
  \colon    \Ccat(X', G(-))
  \to       \Ccat(X, G(-)) \,.
\]
The image of~$F'$ is by assumption contained in the full subcategory~$\Ecat$ of~$\Fun(\Dcat, \Set)$;
we may therefore regard~$F'$ instead as a functor~$F' \colon \Ccat \to \Ecat$.

We now define the desired left adjoint~$F \colon \Ccat \to \Dcat$ as the composition
\[
    F
  \colon
    \Ccat
  \xlongto{F'}
    \Ecat
  \xlongto{E'}
    \Dcat \,.
\]
That~$F$ is indeed left adjoint to~$G$ follows from the computation
\begin{align*}
          \Dcat(F(-_1), -_2)
  &=      (E \circ F)(-_1)(-_2)
   =      (E \circ E' \circ F')(-_1)(-_2) \\
  &\cong  (\Id_\Ecat \circ F')(-_1)(-_2)
   =      F'(-_1)(-_2)
   =      \Ccat(-_1, G(-_2)) \,.
\end{align*}




