\section{}





\subsection{}

The adjunction is given by the natural bijections
\[
          \varphi_{V,M}
  \colon  (\Modl{A})(A \tensor_k V, M)
  \to     (\Modl{k})(V, G(M))
\]
which are given by
\[
    \varphi_{V,M}(f)(v)
  = f(1 \tensor v)
  \qquad\text{and}\qquad
    \varphi_{V,M}^{-1}(g)(a \tensor v)
  = a g(m) \,.
\]
It follows that the unit~$\eta \colon \Id_{\Modl{A}} \to G \circ F$ is at an object~$V \in \Ob(\Modl{k})$ given by
\[
          \eta_V
  =       \varphi_{V, A \tensor_k V}( \id_{A \tensor_k V} )
  \colon  V
  \to     A \tensor_k V \,,
  \\
          v
  \mapsto 1 \tensor v \,,
\]
and that the counit~$\varepsilon \colon F \circ G \to \Id_{\Modl{k}}$ is at an object~$M \in \Ob(\Modl{A})$ given by
\[
            \varepsilon_M
  =         \varphi_{G(M),M}^{-1}( \id_{G(M)} )
  \colon    A \tensor_k G(M)
  \to       M \,,
  \quad     a \tensor m
  \mapsto   a m \,.
\]




\subsection{}

The adjunction is given by the natural bijections
\[
          \varphi_{M,P}
  \colon  (\Modr{B})(M \tensor_A N, P)
  \to     (\Modr{A})(M, \Hom_B(N, P))
\]
which are given by
\[
    \varphi_{M,P}(f)(m)(n)
  = f(m \tensor n)
  \qquad\text{and}\qquad
    \varphi_{M,P}^{-1}(g)(m \tensor n)
  = g(m)(n) \,.
\]
It follows that the unit~$\eta \colon \Id_{\Modr{A}} \to G \circ F$ is at an object~$M$ given by
\begin{align*}
            \eta_M
   =        \varphi_{M, M \tensor_A N}( \id_{M \tensor_A N} )
   \colon   M
  &\to      \Hom_B(N, M \tensor_A N) \,,
  \\
            m
  &\mapsto  (n \mapsto m \tensor n) \,,
\end{align*}
and that the counit~$\varepsilon \colon F \circ G \to \Id_{\Modr{B}}$ is at an object~$P$ given by
\begin{align*}
            \varepsilon_P
   =        \varphi_{\Hom_B(N,P), P}^{-1}( \id_{\Hom_B(N,P)} )
   \colon   \Hom_B(N, P) \tensor_A N
  &\to      P \,,
    \\       
            g \tensor n
  &\mapsto  g(n) \,.
\end{align*}





\subsection{}

The adjunction is given by the natural bijections
\[
          \varphi_{(A,S), B}
  \colon  \CommRing(S^{-1} A, B)
  \to     \Ccat((A,S), (B,B^\times)) \,,
\]
which are given by
\[
    \varphi_{(A,S),B}(f)
  = f \circ i_{A,S}
  \quad\text{and}\quad
    \varphi_{(A,S),B}^{-1}\left( \frac{a}{s} \right)
  = f(a) f(s)^{-1} \,,
\]
where~$i_{A,S} \colon A \to S^{-1} A$,~$a \mapsto a/1$ denotes the canonical homomorphism.
It follows that the unit~$\eta \colon \Id_{\Ccat} \to G \circ F$ is at an object~$(A,S)$ given by
\[
            \eta_{(A,S)}
  =         \varphi_{(A,S), S^{-1} A}
  \colon    ( A, S )
  \to       ( S^{-1} A, (S^{-1} A)^\times ) \,,
  \quad     \eta_{(A,S)}
  =         i_{A,S} \,,
\]
and that the counit~$\varepsilon \colon F \circ G \to \Id_{\CommRing}$ is at an object~$B$ given by
\[
            \varepsilon_{(B^\times)^{-1} B}
  =         \varphi_{(B^\times)^{-1} B, B}( \id_{(B,B^\times)} )
  \colon    (B^\times)^{-1} B
  \to       B \,,
  \quad     \frac{b}{u}
  \mapsto   b u^{-1} \,.
\]




